ProgramDerivation: adding caches

ProgramDerivation.v
@@ -501,3 +501,106 @@ Definition derived_counter : { counter' | adt_refine counter counter' }.
 Defined.
   
 Eval simpl in proj1_sig derived_counter.
+
+
+(** * Another refinement strategy: introducing a cache (a.k.a. finite differencing) *)
+
+Inductive CachingMethods {state} (name : string) (func : state -> nat)
+  : forall {names}, methods state names -> methods (state * nat) names -> Prop :=
+| CmNil :
+    CachingMethods name func MethodsNil MethodsNil
+| CmCached : forall names (ms1 : methods state names) (ms2 : methods _ names),
+    CachingMethods name func ms1 ms2
+    -> CachingMethods name func
+       (MethodsCons {| MethodName := name; MethodBody := (fun s _ => ret (s, func s)) |} ms1)
+       (MethodsCons {| MethodName := name; MethodBody := (fun s arg => ret (s, snd s)) |} ms2)
+| CmDefault : forall name' names oldbody (ms1 : methods state names) (ms2 : methods _ names),
+    name' <> name
+    -> CachingMethods name func ms1 ms2
+    -> CachingMethods name func
+       (MethodsCons {| MethodName := name'; MethodBody := oldbody |} ms1)
+       (MethodsCons {| MethodName := name'; MethodBody := (fun s arg =>
+                         p <- oldbody (fst s) arg;
+                         new_cache <- pick c where (func (fst s) = snd s -> func (fst p) = c);
+                         ret ((fst p, new_cache), snd p)) |} ms2).
+
+Lemma CachingMethods_ok  : forall state name (func : state -> nat)
+                                  names (ms1 : methods state names) (ms2 : methods (state * nat) names),
+    CachingMethods name func ms1 ms2
+    -> RefineMethods (fun s1 s2 => fst s2 = s1 /\ snd s2 = func s1) ms1 ms2.
+Proof.
+  induct 1; eauto.
+
+  econstructor; eauto.
+  unfold ret, bind.
+  simplify; first_order; subst.
+  invert H1.
+  rewrite H2.
+  eauto.
+
+  econstructor; eauto.
+  unfold ret, bind.
+  simplify; first_order; subst.
+  invert H5.
+  unfold pick_ in H4.
+  cases x; simplify.
+  eauto.
+Qed.
+
+Hint Resolve CachingMethods_ok.
+
+Theorem refine_cache : forall state name (func : state -> nat)
+                            names (ms1 : methods state names) (ms2 : methods (state * nat) names)
+                            constr,
+    CachingMethods name func ms1 ms2
+    -> adt_refine {| AdtState := state;
+                     AdtConstructor := constr;
+                     AdtMethods := ms1 |}
+                  {| AdtState := state * nat;
+                     AdtConstructor := s0 <- constr; ret (s0, func s0);
+                     AdtMethods := ms2 |}.
+Proof.
+  simplify.
+  choose_relation (fun s1 s2 => fst s2 = s1 /\ snd s2 = func s1); eauto.
+
+  unfold bind, ret in *.
+  first_order; subst.
+  simplify; eauto.
+Qed.
+
+Ltac refine_cache nam := eapply refine_trans; [ eapply refine_cache with (name := nam);
+   repeat (apply CmNil
+           || refine (CmCached _ _ _ _ _ _)
+           || (refine (CmDefault _ _ _ _ _ _ _ _ _); [ equality | ])) | ].
+
+(** ** An example with lists of numbers *)
+
+Definition sum := fold_right plus 0.
+
+Definition nats := ADT {
+  rep = list nat
+  and constructor = ret []
+  and method "add"[[self, n]] = ret (n :: self, 0)
+  and method "sum"[[self, _]] = ret (self, sum self)
+}.
+
+Definition optimized_nats : { nats' | adt_refine nats nats' }.
+  unfold nats; eexists.
+
+  refine_cache "sum".
+
+  refine_constructor.
+  rewrite bind_ret.
+  finish.
+
+  refine_method "add".
+  rewrite bind_ret; simplify.
+  rewrite (pick_one (arg + snd s)).
+  rewrite bind_ret.
+  finish.
+  equality.
+
+  refine_finish.
+Defined.
+
+Eval simpl in proj1_sig optimized_nats.
